minuska-examples/theories/dep.v
@@ -1,0 +1,20 @@
+Require dpdgraph.dpdgraph.
+
+(* From Coq Require Classes.Morphisms. *)
+
+From Minuska Require naive_interpreter.
+From MinuskaExamples Require examples.
+
+(*Print DependGraph examples.fib_native.interp_from.
+
+Print All Dependencies examples.fib_native.interp_from.*)
+
+
+Set DependGraph File "naiveinterpreter.dpd".
+
+(* Print FileDependGraph Coq.Classes.Morphisms.trans_co_impl_morphism_obligation_1 examples.my_flag. *)
+(*
+Print DependGraph naive_interpreter.naive_interpreter.
+Print All Dependencies naive_interpreter.naive_interpreter.
+*)
+
