minuska-examples/theories/extraction.v
@@ -36,3 +36,12 @@ Extraction
   "SumToN.ml"
   imp.interp_program_count_to
 .
+
+Extraction
+  "Attempt.ml"
+  fib_native.interp_from
+.
+
+
+
+(* Print DependGraph fib_native.interp_from. *)
